dev/lf/paths/tight/Definitions.v
@@ -21,7 +21,7 @@ Inductive avar : Set :=
   | avar_b : nat -> avar  (* bound var (de Bruijn index) *)
   | avar_f : var -> avar. (* free var ("name"), refers to store or ctx *)
 
-Inductive pathmode: Set := strong | general.
+Inductive pathmode: Set := strong | gen.
 
 Inductive typ : Set :=
   | typ_top  : typ
@@ -340,8 +340,12 @@ Inductive ty_trm : ctx -> trm -> typ -> Prop :=
     (forall x, x \notin L ->
       G && x ~ T ||^ x |- ds |||^ x ::: T ||^ x) ->
     G |- trm_val (val_new T ds) :: typ_bnd T
-| ty_fld_elim : forall G p a m T,
-    G |- trm_path p :: typ_rcd {{ a [m] T }} ->
+| ty_fld_elim_var : forall G x a T,
+    G |- trm_path (p_var (avar_f x)) :: typ_rcd {{ a [gen] T }} ->
+    G |- trm_path (p_sel (p_var (avar_f x)) a) :: T
+| ty_fld_elim_path : forall G p a T,
+    G |- trm_path p :: typ_rcd {{ a [strong] T }} ->
+    norm G p ->
     G |- trm_path (p_sel p a) :: T
 | ty_let : forall L G t u T U,
     G |- t :: T ->
@@ -369,7 +373,7 @@ with ty_def : ctx -> var -> typ -> def -> dec -> Prop := (* Γ; z: U |- d: T U *
     G && x ~ U |- def_typ A T :: dec_typ A T T
 | ty_def_trm : forall x G a t T U,
     G & x ~ U |- t :: T ->
-    G && x ~ U |- def_trm a t :: {{ a [general] T }}
+    G && x ~ U |- def_trm a t :: {{ a [gen] T }}
 | ty_def_path : forall x G a p U T,
     G |- trm_path p :: T ->
     norm G p ->
@@ -421,7 +425,7 @@ with subtyp : ctx -> typ -> typ -> Prop :=
     G |- S <: typ_and T U
 | subtyp_fld: forall G a T U,
     G |- T <: U ->
-    G |- typ_rcd {{ a [general] T }} <: typ_rcd {{ a [general] U }}
+    G |- typ_rcd {{ a [gen] T }} <: typ_rcd {{ a [gen] U }}
 | subtyp_typ: forall G A S1 T1 S2 T2,
     G |- S2 <: S1 ->
     G |- T1 <: T2 ->
@@ -440,7 +444,7 @@ with subtyp : ctx -> typ -> typ -> Prop :=
        G & x ~ S2 |- T1 ||^ x <: T2 ||^ x) ->
     G |- typ_all S1 T1 <: typ_all S2 T2
 | subtyp_path: forall G a T,
-    G |- typ_rcd {{ a [strong] T }} <: typ_rcd {{ a [general] T }}
+    G |- typ_rcd {{ a [strong] T }} <: typ_rcd {{ a [gen] T }}
 where "G '|-' T '<:' U" := (subtyp G T U).
 
 Reserved Notation "G '|-!' t '::' T" (at level 40, t at level 59).
@@ -460,8 +464,9 @@ Inductive ty_trm_p : ctx -> trm -> typ -> Prop :=
 | ty_rec_elim_p : forall G p T,
     G |-! trm_path p :: typ_bnd T ->
     G |-! trm_path p :: open_typ_p p T
-|ty_fld_elim_p : forall G p a m T,
-    G |-! trm_path p :: typ_rcd {{ a [m] T }} ->
+|ty_fld_elim_p : forall G p a T,
+    G |-! trm_path p :: typ_rcd {{ a [strong] T }} ->
+    norm G p ->
     inert_typ T ->
     G |-! trm_path (p_sel p a) :: T
 | ty_and1_p : forall G p T U,
@@ -493,8 +498,12 @@ Inductive ty_trm_t : ctx -> trm -> typ -> Prop :=
     (forall x, x \notin L ->
       G && x ~ T ||^ x |- ds |||^ x ::: T ||^ x) ->
     G |-# trm_val (val_new T ds) :: typ_bnd T
-| ty_fld_elim_t : forall G p a m T,
-    G |-# trm_path p :: typ_rcd {{ a [m] T }} ->
+| ty_fld_elim_var_t : forall G x a T,
+    G |-# trm_path (p_var (avar_f x)) :: typ_rcd {{ a [gen] T }} ->
+    G |-# trm_path (p_sel (p_var (avar_f x)) a) :: T
+| ty_fld_elim_path_t : forall G p a T,
+    G |-# trm_path p :: typ_rcd {{ a [strong] T }} ->
+    norm_t G p ->
     G |-# trm_path (p_sel p a) :: T
 | ty_let_t : forall L G t u T U,
     G |-# t :: T ->
@@ -548,7 +557,7 @@ with subtyp_t : ctx -> typ -> typ -> Prop :=
     G |-# S <: typ_and T U
 | subtyp_fld_t: forall G a T U,
     G |-# T <: U ->
-    G |-# typ_rcd {{ a [general] T }} <: typ_rcd {{ a [general] U }}
+    G |-# typ_rcd {{ a [gen] T }} <: typ_rcd {{ a [gen] U }}
 | subtyp_typ_t: forall G A S1 T1 S2 T2,
     G |-# S2 <: S1 ->
     G |-# T1 <: T2 ->
@@ -567,7 +576,7 @@ with subtyp_t : ctx -> typ -> typ -> Prop :=
        G & x ~ S2 |- T1 ||^ x <: T2 ||^ x) ->
     G |-# typ_all S1 T1 <: typ_all S2 T2
 | subtyp_path_t: forall G a T,
-    G |-# typ_rcd {{ a [strong] T }} <: typ_rcd {{ a [general] T }}
+    G |-# typ_rcd {{ a [strong] T }} <: typ_rcd {{ a [gen] T }}
 where "G '|-#' T '<:' U" := (subtyp_t G T U).
 
 Reserved Notation "G '~~' s" (at level 40).
